<div style="float: left; width: 64%; padding: 1%;">

## äºŒã€ğŸŒŸå‘é‡çš„è¿ç®—

<ul>

ï¼ˆä»¥ $\mathbf{R}^{3}$ ä¸ºä¾‹ï¼‰è®° $a=\left(a_{1}, a_{2}, a_{3}\right), b=\left(b_{1}, b_{2}, b_{3}\right), c=\left(c_{1}, c_{2}, c_{3}\right)$ï¼Œåˆ™

1. **å‘é‡çš„åŠ å‡è¿ç®—**ï¼š

   $$
   a \pm b=\left(a_{1} \pm b_{1}\right) i+\left(a_{2} \pm b_{2}\right) j+\left(a_{3} \pm b_{3}\right) k
   $$

2. **æ•°ä¹˜è¿ç®—**ï¼š

   $$
   \lambda a=\lambda a_{1} i+\lambda a_{2} j+\lambda a_{3} k
   $$

3. **æ•°é‡ç§¯**ï¼š

   - ä»£æ•°è¡¨ç¤ºï¼š

     $$
     a \cdot b=a_{1} b_{1}+a_{2} b_{2}+a_{3} b_{3}
     $$

   - å‡ ä½•è¡¨ç¤ºï¼š

     $$
     a \cdot b=|a| |b| \cos \theta
     $$

   - è¿ç®—è§„å¾‹ï¼š
     - äº¤æ¢å¾‹ï¼š$a \cdot b=b \cdot a$
     - åˆ†é…å¾‹ï¼š$a \cdot(b+c)=a \cdot b+a \cdot c$

   - å‡ ä½•åº”ç”¨ï¼š
     - æ±‚æ¨¡ï¼š$|a|=\sqrt{a \cdot a}$
     - æ±‚å¤¹è§’ï¼š$\cos \theta=\frac{a \cdot b}{|a||b|}$
     - åˆ¤å®šä¸¤å‘é‡å‚ç›´ï¼š$\boldsymbol{a} \perp \boldsymbol{b} \Leftrightarrow \boldsymbol{a} \cdot \boldsymbol{b}=0$

4. ğŸŒŸ**å‘é‡ç§¯**ï¼š

   - ä»£æ•°è¡¨ç¤ºï¼š

     $$
     \boldsymbol{a} \times \boldsymbol{b}=\left|\begin{array}{ccc}i & j & k \\ a_{1} & a_{2} & a_{3} \\ b_{1} & b_{2} & b_{3}\end{array}\right|
     $$

   - è¿ç®—è§„å¾‹ï¼š

     $$
     \boldsymbol{a} \times \boldsymbol{b}=-(b \times \boldsymbol{a})
     $$

     $$
     a \times(b+c)=a \times b+a \times c
     $$

   - å‡ ä½•åº”ç”¨ï¼š
     - æ±‚åŒæ—¶å‚ç›´äº $a$ å’Œ $b$ çš„å‘é‡ï¼š$a \times b$
     - æ±‚ä»¥ $a$ å’Œ $b$ ä¸ºé‚»è¾¹çš„å¹³è¡Œå››è¾¹å½¢é¢ç§¯ï¼š$S=|\boldsymbol{a} \times \boldsymbol{b}|$
     - åˆ¤å®šä¸¤å‘é‡å¹³è¡Œï¼š$\boldsymbol{a} // \boldsymbol{b} \Leftrightarrow \boldsymbol{a} \times \boldsymbol{b}=\mathbf{0}$

5. **æ··åˆç§¯**ï¼š

   $$
   (\boldsymbol{a} \boldsymbol{b} \boldsymbol{c})=(\boldsymbol{a} \times \boldsymbol{b}) \cdot \boldsymbol{c}=\left|\begin{array}{lll}a_{1} & a_{2} & a_{3} \\ b_{1} & b_{2} & b_{3} \\ c_{1} & c_{2} & c_{3}\end{array}\right|
   $$

   - è¿ç®—è§„å¾‹ï¼š

     $$
     (\boldsymbol{a} \boldsymbol{b} \boldsymbol{c})=(\boldsymbol{b} \boldsymbol{c} \boldsymbol{a})=(\boldsymbol{c} \boldsymbol{a} \boldsymbol{b})
     $$

     $$
     (\boldsymbol{a} \boldsymbol{b} \boldsymbol{c})=-(a c b)
     $$

   - å‡ ä½•åº”ç”¨ï¼š
     - æ±‚ä»¥ $\boldsymbol{a}, \boldsymbol{b}, \boldsymbol{c}$ ä¸ºæ£±çš„å¹³è¡Œå…­é¢ä½“ä½“ç§¯ï¼š$V_{\text{å¹³è¡Œå…­é¢ä½“}}=|(\boldsymbol{a} \boldsymbol{b} \boldsymbol{c})|$
     - åˆ¤å®šä¸‰å‘é‡å…±é¢ï¼š$\boldsymbol{a}, \boldsymbol{b}, \boldsymbol{c}$ å…±é¢ $\Leftrightarrow (\boldsymbol{a} \boldsymbol{b} \boldsymbol{c})=0$

</ul>

</ul>
</div>
<div style="float: right; width: 26%; padding: 1%;">

</div>
<div style="clear: both;"></div>
