<div style="float: left; width: 64%; padding: 1%;">

### 非齐次线性方程的通解结构

<ul>

设 $y^{*}(x)$ 为 (1) 的一个解，$Y(x)$ 为 (1) 对应的 (2) 的通解，则

$$
y=Y(x)+y^{*}(x)
$$

为 (1) 的通解。

**定理（自由项为 $f(x)=f_{1}(x)+f_{2}(x)$ 的解的叠加原理）**  
设 $y_{i}^{*}$ 为

$$
y^{(n)}+a_{1}(x) y^{(n-1)}+\cdots+a_{n-1}(x) y^{\prime}+a_{n}(x) y=f_{i}(x)
$$

的解 $(i=1,2)$，则 $y_{1}^{*}(x)+y_{2}^{*}(x)$ 为

$$
y^{(n)}+a_{1}(x) y^{(n-1)}+\cdots+a_{n-1}(x) y^{\prime}+a_{n}(x) y=f_{1}(x)+f_{2}(x)
$$

的解。

</ul>
</div>
<div style="float: right; width: 26%; padding: 1%;">

</div>
<div style="clear: both;"></div>
